{
 "cells": [
  {
   "cell_type": "markdown",
   "id": "0446e4eb-5794-41d5-aef4-1dea3a7bb988",
   "metadata": {
    "tags": []
   },
   "source": [
    "# Exercise \\#2\n",
    "*Jacob Oliver Bruun*"
   ]
  },
  {
   "cell_type": "markdown",
   "id": "1b593b20-47e0-4497-ba2e-2543b132039b",
   "metadata": {},
   "source": [
    "## Problem 1"
   ]
  },
  {
   "cell_type": "markdown",
   "id": "c23d6916-27e4-41f6-8cec-2dccdd7198d7",
   "metadata": {},
   "source": [
    "### a)\n",
    "\n",
    "Let $f(x) = \\sin 6\\pi x + \\cos 2\\pi x$, we can clearly see that $f$ is its own real Fourier series. For its exponential form, we have\n",
    "$$\n",
    "f(x) = \\frac{1}{2} \\left( ie^{-6i\\pi x} - ie^{6i \\pi x} + e^{-2i\\pi x} + e^{2i\\pi x} \\right)\n",
    "$$\n",
    "which is its exponential Fourier series."
   ]
  },
  {
   "cell_type": "markdown",
   "id": "c1488dfa-b868-4f66-83e4-acfb5d81b870",
   "metadata": {},
   "source": [
    "### b)\n",
    "\n",
    "Let $f(x) = 3\\sin^2 x + 3 \\cos^2 x$, we can find\n",
    "$$\n",
    "f(x) = 3\\left( \\sin^2 x + \\cos^2 \\right) = 3\n",
    "$$\n",
    "which is its own Fourier series."
   ]
  },
  {
   "cell_type": "markdown",
   "id": "832067ac-4190-41eb-9f77-44f78d37f705",
   "metadata": {},
   "source": [
    "### c)\n",
    "\n",
    "Let $f(x) = x + x^2/2$, we can see that $x$ is odd and $x^2/2$ is even and can find their corresponing sine and cosine series.\n",
    "$$\n",
    "\\begin{split}\n",
    "b_k = \\int_{-1/2}^{1/2} x\\sin (2\\pi kx) dx\n",
    "&= \\left[ -\\frac{x}{2\\pi k} \\cos(2\\pi kx) \\right]_{-1/2}^{1/2} + \\frac{1}{2\\pi k} \\int_{-1/2}^{1/2} \\cos(2\\pi kx)dx \\\\\n",
    "&= -\\frac{1}{4\\pi k} \\left[ \\cos(\\pi k) + \\cos(-\\pi k) \\right] + \\frac{1}{2\\pi k} \\left[ \\frac{\\sin(2\\pi kx)}{2\\pi k} \\right]_{-1/2}^{1/2} \\\\\n",
    "&= -\\frac{(-1)^k}{2\\pi k} + \\frac{1}{4\\pi^2 k^2} \\left[ \\sin(\\pi k) - \\sin(-\\pi k) \\right] \\\\\n",
    "&= -\\frac{(-1)^k}{2\\pi k}\n",
    "\\end{split}\n",
    "$$\n",
    "and\n",
    "$$\n",
    "\\begin{split}\n",
    "a_k = \\int_{-1/2}^{1/2} \\frac{x^2}{2} \\cos(2\\pi kx) dx\n",
    "&= \\left[ \\frac{x^2}{4\\pi k} \\sin(2\\pi kx) \\right]_{-1/2}^{1/2} - \\frac{1}{2\\pi k} \\int_{-1/2}^{1/2} x\\sin(2\\pi kx)dx \\\\\n",
    "&= \\frac{(-1)^k}{4\\pi^2 k^2}\n",
    "\\end{split}\n",
    "$$\n",
    "lastly\n",
    "$$\n",
    "a_0 = \\int_{-1/2}^{1/2} \\left( x + \\frac{x^2}{2} \\right) dx = \\left[ \\frac{x^2}{2} + \\frac{x^3}{6} \\right]_{-1/2}^{1/2} = \\frac{2}{8} + \\frac{2}{48} = \\frac{7}{24}\n",
    "$$\n",
    "and we have the Fourier series\n",
    "$$\n",
    "f(x) = \\frac{7}{24} + \\sum_{k=1}^\\infty \\frac{(-1)^k}{2\\pi k} \\sin(2\\pi kx) + \\sum_{k=1}^\\infty \\frac{(-1)^k}{4\\pi^2 k^2} \\cos(2\\pi kx).\n",
    "$$\n",
    "We now find the exponential form by\n",
    "$$\n",
    "\\begin{split}\n",
    "c_k &= \\int_{-1/2}^{1/2} \\left( x + \\frac{x^2}{2} \\right) e^{2\\pi ikx} dx \\\\\n",
    "&= \\left[ \\left( x + \\frac{x^2}{2} \\right) \\frac{1}{2\\pi ik} e^{2\\pi ikx} \\right]_{-1/2}^{1/2} - \\frac{1}{2\\pi ik} \\int_{-1/2}^{1/2} (1 + x) e^{2\\pi ikx} dx \\\\\n",
    "&= \\frac{5}{16\\pi ik} e^{\\pi ik} - \\frac{3}{16\\pi ik}e^{-\\pi ik} - \\frac{1}{2\\pi ik} \\left( \\left[ \\frac{1+x}{2\\pi ik} e^{2\\pi ikx} \\right]_{-1/2}^{1/2} - \\int_{-1/2}^{1/2} e^{2\\pi ikx} dx \\right) \\\\\n",
    "&= \\frac{5}{16\\pi ik} e^{\\pi ik} - \\frac{3}{16 \\pi ik} e^{-\\pi ik} + \\frac{3}{8 \\pi^2 k^2} e^{\\pi ik} + \\frac{1}{8 \\pi^2 k^2} e^{-\\pi ik} + \\frac{1}{2\\pi ik} \\left[ \\frac{1}{2\\pi ik} e^{2\\pi ikx} \\right]_{-1/2}^{1/2} \\\\\n",
    "&= \\frac{5}{16\\pi ik} e^{\\pi ik} - \\frac{3}{16 \\pi ik} e^{-\\pi ik} + \\frac{3}{8 \\pi^2 k^2} e^{\\pi ik} + \\frac{1}{8 \\pi^2 k^2} e^{-\\pi ik} - \\frac{1}{4\\pi^2 k^2} e^{\\pi ik} - \\frac{1}{4\\pi^2 k^2} e^{-\\pi ik} \\\\\n",
    "&= \\frac{(-1)^k}{8\\pi ik}\n",
    "\\end{split}\n",
    "$$\n",
    "as $e^{\\pi ik} = e^{-\\pi ik} = (-1)^k, \\; \\forall k \\in \\mathbb{Z}$. We then have the exponential Fourier series\n",
    "$$\n",
    "f(x) = \\sum_{k\\in \\mathbb{Z}} \\frac{(-1)^k}{8\\pi ik} e^{2\\pi ikx}\n",
    "$$"
   ]
  },
  {
   "cell_type": "markdown",
   "id": "cb8985cb-a98f-43a9-b1ac-23903882e280",
   "metadata": {},
   "source": [
    "### d)\n",
    "\n",
    "Let $f(x) = e^{-2\\pi x}$ We now check\n",
    "$$\n",
    "c_k = \\int_{-1/2}^{1/2} e^{-2\\pi x} e^{2\\pi ikx} dx\n",
    "= \\int_{-1/2}^{1/2} e^{2\\pi(ik - 1)x} dx\n",
    "= \\frac{1}{2\\pi(ik-1)} \\left[ e^{2\\pi(ik-1)x} \\right]_{-1/2}^{1/2} = \\frac{e^{\\pi ik} e^{-\\pi} - e^{-\\pi ik} e^{\\pi}}{2\\pi (ik-1)} = \\frac{(-1)^k \\left( e^{-\\pi} - e^{\\pi} \\right)}{2\\pi (ik-1)}.\n",
    "$$\n",
    "we then have the exponential Fourier series\n",
    "$$\n",
    "f(x) = \\sum_{k\\in \\mathbb{Z}} \\frac{(-1)^k \\left( e^{-\\pi} - e^{\\pi} \\right)}{2\\pi (ik-1)} e^{2\\pi ikx}\n",
    "$$\n",
    "We can find the trigonometric Fourier series by\n",
    "$$\n",
    "a_k = c_k + c_{-ik}, \\;\\; b_k = i\\left( c_k - c_{-k} \\right)\n",
    "$$"
   ]
  },
  {
   "cell_type": "markdown",
   "id": "f3144b5b-b882-4f6f-a15f-6165ed4410b8",
   "metadata": {},
   "source": [
    "## Problem 2"
   ]
  },
  {
   "cell_type": "markdown",
   "id": "698a129e-4772-44aa-a79a-0a6812c719f3",
   "metadata": {},
   "source": [
    "### a)\n",
    "\n",
    "Let an inner product be defined by\n",
    "$$\n",
    "\\left< f, g \\right> = \\int_0^1 x f(x)g(x) dx.\n",
    "$$\n",
    "Now let $V = \\left\\lbrace \\mathbf{v}_1, \\mathbf{v}_2, \\dots \\right\\rbrace$ be the monomial basis and let $U = \\left\\lbrace \\mathbf{u}_1, \\dots \\mathbf{u}_n \\right\\rbrace$ be an orthonormal basis of $\\mathcal{P}$. Let $\\mathbf{u}_1 = 1$. We now use the Gram-Schmidt process to find $\\mathbf{u}_2, \\mathbf{u}_3$.\n",
    "$$\n",
    "\\mathbf{u}_2 = \\mathbf{v}_2 - \\frac{\\left< \\mathbf{v}_2, \\mathbf{u}_1 \\right>}{\\left< \\mathbf{u}_1, \\mathbf{u}_1 \\right>} \\mathbf{u}_1 = x - \\frac{\\left< x, 1 \\right>}{\\left< 1, 1 \\right>}\\cdot 1\n",
    "$$\n",
    "we find\n",
    "$$\n",
    "\\begin{split}\n",
    "\\left< 1, 1 \\right> &= \\int_0^1 x dx = \\frac{1}{2} \\\\\n",
    "\\left< x, 1 \\right> &= \\int_0^1 x^2 dx = \\frac{1}{3}\n",
    "\\end{split}\n",
    "$$\n",
    "thus\n",
    "$$\n",
    "\\mathbf{u}_2 = x - \\frac{2}{3}\n",
    "$$\n",
    "further\n",
    "$$\n",
    "\\mathbf{u}_3 = x^2 - \\frac{\\left< x^2, 1 \\right>}{\\left< 1, 1 \\right>} - \\frac{\\left< x^2, x - 2/3 \\right>}{\\left< x - 2/3, x - 2/3 \\right>} x\n",
    "$$\n",
    "we now can find\n",
    "$$\n",
    "\\begin{split}\n",
    "\\left< x^2, 1 \\right> &= \\int_0^1 x^3 dx = \\frac{1}{4} \\\\\n",
    "\\left< x^2, x - 2/3 \\right> &= \\int_0^1 \\left( x^4 - \\frac{2}{3} x^3 \\right) dx = \\frac{1}{5} - \\frac{2}{12} = \\frac{1}{30} \\\\\n",
    "\\left< x - 2/3, x - 2/3 \\right> &= \\int_0^1 \\left( x^2 - \\frac{4}{3}x + \\frac{4}{9} \\right) dx = \\frac{1}{3} - \\frac{2}{3} + \\frac{4}{9} = \\frac{1}{9}\n",
    "\\end{split}\n",
    "$$\n",
    "thus\n",
    "$$\n",
    "\\mathbf{u}_3 = x^2 - \\frac{9}{30} \\left( x - \\frac{2}{3} \\right) - \\frac{1}{2} = x^2 - \\frac{9}{30}x - \\frac{9}{30}.\n",
    "$$"
   ]
  },
  {
   "cell_type": "markdown",
   "id": "a6546457-3b44-4251-92e2-cd3995672958",
   "metadata": {},
   "source": [
    "### b)\n",
    "\n",
    "Let an inner product be defined by\n",
    "$$\n",
    "\\left< f, g \\right> = \\int_0^\\infty e^{-x} f(x) g(x) dx.\n",
    "$$\n",
    "By the same assumptions as the last task, $\\mathbf{u}_1 = 1$ and\n",
    "$$\n",
    "\\mathbf{u}_2 = x - \\frac{\\left< x, 1 \\right>}{\\left< 1, 1 \\right>}\n",
    "$$\n",
    "we find\n",
    "$$\n",
    "\\begin{split}\n",
    "\\left< 1, 1 \\right> &= \\int_0^\\infty e^{-x} dx = \\left[ -e^{-x} \\right]_0^\\infty = 1 \\\\\n",
    "\\left< x, 1 \\right> &= \\int_0^\\infty xe^{-x} dx = \\left[ -x e^{-x} \\right]_0^\\infty + \\int_0^\\infty e^{-x} dx = 1 \\\\\n",
    "\\end{split}\n",
    "$$\n",
    "thus\n",
    "$$\n",
    "\\mathbf{u}_2 = x-1.\n",
    "$$\n",
    "The third polynomial $\\mathbf{u}_3$ must be orthogonal to both $\\mathbf{u}_1, \\mathbf{u}_2$, and normal. Let $\\mathbf{u}_3 = x^2 - 4x + 2$, now firstly we can see\n",
    "$$\n",
    "\\int_0^\\infty x^n e^{-x} dx = n!\n",
    "$$\n",
    "then\n",
    "$$\n",
    "\\begin{split}\n",
    "\\left< x^2 - 4x + 2, 1 \\right> &= \\int_0^\\infty \\left( x^2 - 4x + 2 \\right) e^{-x} dx = 2 - 4 + 2 = 0 \\\\\n",
    "\\left< x^2 - 4x + 2, x - 1 \\right> &= \\int_0^\\infty \\left( x^3 - 5x^2 + 6x - 2 \\right) e^{-x} dx = 6 - 10 + 6 - 2 = 0.\n",
    "\\end{split}\n",
    "$$\n",
    "$\\mathbf{u}_3 = x^2 - 4x + 2$ is therefore the third polynomial."
   ]
  },
  {
   "cell_type": "markdown",
   "id": "468676fc-a80c-42ab-90c3-0e36a8ef9936",
   "metadata": {},
   "source": [
    "### c)\n",
    "\n",
    "Let\n",
    "$$\n",
    "h(x) = \\left\\lbrace \\begin{array}{l l} 1, & x\\in \\left[ 0, 1 \\right], \\\\ 0, & \\text{else.} \\end{array} \\right.\n",
    "$$\n",
    "we now find the generalised Fourier coefficients\n",
    "$$\n",
    "\\begin{split}\n",
    "c_0 &= \\frac{\\left< h, 1 \\right>}{\\left< 1, 1 \\right>} = \\int_0^1 e^{-x} dx = 1-e^{-1} \\\\\n",
    "c_1 &= \\frac{\\left< h, x-1 \\right>}{\\left< x-1, x-1 \\right>} = \\frac{\\int_0^1 (x-1)e^{-x} dx}{\\int_0^\\infty \\left( x^2 - 2x + 1 \\right) e^{-x} dx} = \\left[ -(x-1)e^{-x} \\right]_0^1 + \\int_0^1 e^{-x} dx = -e^{-1} \\\\\n",
    "c_2 &= \\frac{\\left< h, x^2 - 4x + 2 \\right>}{\\left< x^2 - 4x + 2, x^2 - 4x + 2 \\right>}\n",
    "= \\frac{\\int_0^1 \\left( x^2 - 4x + 2 \\right)e^{-x} dx}{\\int_0^\\infty \\left( x^4 - 8x^3 + 20x^2 - 16x + 4 \\right) e^{-x} dx } = \\frac{ \\left[ -\\left( x^2 - 4x + 2 \\right)e^{-x} \\right]_0^1 + 2\\int_0^1 (x-2) e^{-x} dx }{ 24 - 48 + 40 - 16 + 4 } = \\frac{ e^{-1} + 2 + 2 \\left[ -(x-2)e^{-x} \\right]_0^1 + 2\\int_0^1 e^{-x} dx}{4}\n",
    "= \\frac{1}{4}e^{-1}.\n",
    "\\end{split}\n",
    "$$\n",
    "We then get that the closest second degree polynomial to $h(x)$ is\n",
    "$$\n",
    "\\begin{split}\n",
    "Sh(x) &= 1-e^{-1} - e^{-1} \\left( x - 1 \\right) + \\frac{1}{4} e^{-1} \\left( x^2 - 4x + 2 \\right) \\\\\n",
    "&= 1 - xe^{-1} + \\frac{1}{4}x^2 e^{-1} - xe^{-1} + \\frac{1}{2} \\\\\n",
    "&= \\frac{e^{-1}}{4}x^2 - 2e^{-1}x + \\frac{3}{2}\n",
    "\\end{split}\n",
    "$$"
   ]
  },
  {
   "cell_type": "markdown",
   "id": "2f3037ec-5f62-4d9a-91de-27b507eb9be7",
   "metadata": {},
   "source": [
    "## Problem 3"
   ]
  },
  {
   "cell_type": "markdown",
   "id": "95a39605-7575-4b0b-a4ce-9576149d6273",
   "metadata": {},
   "source": [
    "### a)\n",
    "\n",
    "Consider $\\mathcal{P}_2$, the vector space of polynomials with real coefficients of degree 2, with the inner product\n",
    "$$\n",
    "\\left< f(x), g(x) \\right> = \\int_0^1 f(x) g(x) dx.\n",
    "$$\n",
    "lets look at the polynomials\n",
    "$$\n",
    "\\begin{split}\n",
    "p_0 (x) &= 1 \\\\\n",
    "p_1 (x) &= x - \\frac{1}{2} \\\\\n",
    "p_2 (x) &= x^2 - x + \\frac{1}{6} \\\\\n",
    "\\end{split}\n",
    "$$\n",
    "as $p_n$ is a polynomial of degree $n$ they are linearly independent and therefore form a basis of $\\mathcal{P}_2$. We only need to show that it is an orthogonal basis.\n",
    "$$\n",
    "\\begin{split}\n",
    "\\left< p_0, p_1 \\right> &= \\int_0^1 \\left( x - \\frac{1}{2} \\right) dx = 0 \\\\\n",
    "\\left< p_0, p_2 \\right> &= \\int_0^1 \\left( x^2 - x + \\frac{1}{6} \\right) dx = \\frac{1}{3} - \\frac{1}{2} + \\frac{1}{6} = 0 \\\\\n",
    "\\left< p_1, p_2 \\right> &= \\int_0^1 \\left( x^3 - \\frac{3}{2} x^2 + \\frac{2}{3} x - \\frac{1}{12} \\right) dx = \\frac{1}{4} - \\frac{1}{2} + \\frac{1}{3} - \\frac{1}{12} = 0\n",
    "\\end{split}\n",
    "$$\n",
    "thus $\\left\\lbrace p_0, p_1, p_2 \\right\\rbrace$ is a orthogonal basis of $\\mathcal{P}_2$."
   ]
  },
  {
   "cell_type": "markdown",
   "id": "688d63a3-ff31-494e-bca8-dc6c9619ff50",
   "metadata": {},
   "source": [
    "### b)\n",
    "\n",
    "We can write\n",
    "$$\n",
    "p(x) = x^2 = p_2 + p_1 + \\frac{1}{3} p_0.\n",
    "$$"
   ]
  },
  {
   "cell_type": "markdown",
   "id": "69be98fd-b35a-48d6-bfe9-baa1d329ce9e",
   "metadata": {},
   "source": [
    "### c)\n",
    "\n",
    "Let\n",
    "$$\n",
    "A = \\left( \\begin{array}{ccc} 1 & 3 & 0 \\\\ 2 & 8 & 4 \\\\ 1 & 6 & 1 \\\\ \\end{array} \\right)\n",
    "$$\n",
    "define a mapping, $f_A : \\mathcal{P}_2 \\to \\mathcal{P}_2$. We now will find $\\mathbf{y}$ such that $A\\mathbf{y} = \\mathbf{b}$ for $\\mathbf{b}$ the coordinate vector of $p(x)$. We can solve out equation using Gauss elimination.\n",
    "$$\n",
    "\\left[\n",
    "\\begin{array}{ccc|c}\n",
    "    1 & 3 & 0 & 1/3 \\\\\n",
    "    2 & 8 & 4 & 1 \\\\\n",
    "    1 & 6 & 1 & 1 \\\\\n",
    "\\end{array}\n",
    "\\right] \\sim\n",
    "\\left[\n",
    "\\begin{array}{ccc|c}\n",
    "    1 & 3 & 0 & 1/3 \\\\\n",
    "    0 & 1 & 2 & 1/6 \\\\\n",
    "    0 & 3 & 1 & 2/3 \\\\\n",
    "\\end{array}\n",
    "\\right] \\sim\n",
    "\\left[\n",
    "\\begin{array}{ccc|c}\n",
    "    1 & 3 & 0 & 1/3 \\\\\n",
    "    0 & 1 & 2 & 1/6 \\\\\n",
    "    0 & 0 & 1 & -1/30 \\\\\n",
    "\\end{array}\n",
    "\\right] \\sim\n",
    "\\left[\n",
    "\\begin{array}{ccc|c}\n",
    "    1 & 0 & 0 & -11/30 \\\\\n",
    "    0 & 1 & 0 & 7/30 \\\\\n",
    "    0 & 0 & 1 & -1/30 \\\\\n",
    "\\end{array}\n",
    "\\right]\n",
    "$$\n",
    "thus\n",
    "$$\n",
    "\\mathbf{y} = \\left( \\begin{array}{c} -11/30 \\\\ 7/30 \\\\ -1/30 \\end{array} \\right)\n",
    "$$"
   ]
  },
  {
   "cell_type": "markdown",
   "id": "e475b25c-9310-4816-8956-7491401c8009",
   "metadata": {},
   "source": [
    "### d)"
   ]
  },
  {
   "cell_type": "code",
   "execution_count": null,
   "id": "431da549-f37d-4db6-88ae-e4722504905f",
   "metadata": {},
   "outputs": [],
   "source": [
    "from numpy.linalg import solve\n",
    "import numpy as np\n",
    "\n",
    "\n",
    "def linear_equation_solver(A, b):\n",
    "    return solve(A, b)\n",
    "\n",
    "\n",
    "A = np.array([[1, 3, 0], [2, 8, 4], [1, 6, 1]])\n",
    "b = np.array([1/3, 1, 1])\n",
    "\n",
    "ynum = solve(A, b)\n",
    "yanal = [-11/30, 7/30, -1/30]\n",
    "\n",
    "np.allclose(ynum, yanal)"
   ]
  },
  {
   "cell_type": "markdown",
   "id": "a83eb0b4-7292-425a-a4fc-2de5fec53069",
   "metadata": {},
   "source": [
    "## Problem 4"
   ]
  },
  {
   "cell_type": "markdown",
   "id": "6e6e3b13-522f-4a29-8754-c90d83041f8a",
   "metadata": {},
   "source": [
    "### a)"
   ]
  },
  {
   "cell_type": "code",
   "execution_count": null,
   "id": "a19a15c3-a049-4b00-a75b-7c31e3e1ffd3",
   "metadata": {},
   "outputs": [],
   "source": [
    "import matplotlib.pyplot as plt\n",
    "\n",
    "\n",
    "def chebyshev(k, n=100):\n",
    "    x = np.linspace(-1, 1, n)\n",
    "    return np.cos(k*np.arccos(x))\n",
    "\n",
    "\n",
    "x = np.linspace(-1, 1, 100)\n",
    "\n",
    "for k in range(7):\n",
    "    plt.plot(x, chebyshev(k, 100), label=f\"{k=}\")\n",
    "\n",
    "plt.legend()\n",
    "plt.show()\n",
    "\n",
    "\n",
    "def chebyshev_rec(n, x):\n",
    "    if n == 0:\n",
    "        return np.ones(len(x))\n",
    "    elif n == 1:\n",
    "        return x\n",
    "    return 2*x*chebyshev_rec(n-1, x) - chebyshev_rec(n-2, x)\n",
    "\n",
    "\n",
    "for n in range(7):\n",
    "    plt.plot(x, chebyshev_rec(n, x), label=f\"{n=}\")\n",
    "\n",
    "plt.legend()\n",
    "plt.show()"
   ]
  },
  {
   "cell_type": "markdown",
   "id": "31b2e34c-1f3b-48d8-9a47-1192fc792456",
   "metadata": {},
   "source": [
    "### b)"
   ]
  },
  {
   "cell_type": "code",
   "execution_count": null,
   "id": "539965fd-441d-4dcf-8f83-f3a20985f0d2",
   "metadata": {},
   "outputs": [],
   "source": [
    "def cheb_nodes(N):\n",
    "    TN = chebyshev(N, 100)\n",
    "    TN = np.sign(TN)\n",
    "    zeroes = np.zeros(N)\n",
    "    count = 0\n",
    "    for j in range(1, len(TN)):\n",
    "        if TN[j] != TN[j-1]:\n",
    "            zeroes[count] = j\n",
    "            count += 1\n",
    "    return (2*zeroes/len(TN)) -1\n",
    "\n",
    "\n",
    "def cheb_coef(y, t, k):\n",
    "    N = len(t)\n",
    "    ck = 0\n",
    "    if k == 0:\n",
    "        for i in range(N):\n",
    "            ck += y(i)\n",
    "        return ck/N\n",
    "    cheb = chebyshev(k, N)\n",
    "    for i in range(N):\n",
    "        ck += y(i) * cheb[i]\n",
    "    return ck * 2 / N\n",
    "\n",
    "\n",
    "def cheb_interpol(c, s, N):\n",
    "    f = 0\n",
    "    for i in range(N):\n",
    "        f += cheb_coef(c, s, i) * chebyshev(i, len(s))\n",
    "    return f\n",
    "\n",
    "\n",
    "def y(x):\n",
    "    return x**2 + x + 1\n",
    "\n",
    "\n",
    "t = np.linspace(0, 4, 100)\n",
    "cint = cheb_interpol(y, t, 10)\n",
    "\n",
    "plt.plot(t, y(t), label=\"anal\")\n",
    "plt.plot(t, cint, label=\"Fourier\")\n",
    "plt.legend()\n",
    "plt.show()"
   ]
  },
  {
   "cell_type": "markdown",
   "id": "9b20bfac-2f27-43e6-aeaa-6607051a1128",
   "metadata": {},
   "source": [
    "This makes no sense, well well..."
   ]
  }
 ],
 "metadata": {
  "kernelspec": {
   "display_name": "Python 3 (ipykernel)",
   "language": "python",
   "name": "python3"
  },
  "language_info": {
   "codemirror_mode": {
    "name": "ipython",
    "version": 3
   },
   "file_extension": ".py",
   "mimetype": "text/x-python",
   "name": "python",
   "nbconvert_exporter": "python",
   "pygments_lexer": "ipython3",
   "version": "3.11.4"
  }
 },
 "nbformat": 4,
 "nbformat_minor": 5
}
